playground/uart_model/m0u_progScript.sml
@@ -12,6 +12,7 @@ open clockTheory;
 open stateTheory m0_stepTheory;
 open boolSimps;
 open pred_setTheory;
+open sep_helper;
 
 val _ = new_theory "m0u_prog";
 (********************************************)
@@ -19,7 +20,7 @@ val _ = new_theory "m0u_prog";
 (*                                          *)
 (********************************************)
 val _= Datatype `m0u_component = m0_c m0_component
-                               | m0u_c_Input 
+                               | m0u_c_Input
                                | m0u_c_Output
                                | m0u_c_RXD
                                | m0u_c_TXD
@@ -36,15 +37,15 @@ val m0u_proj_def = Define `
 m0u_proj ((s,u),input,output) =
      (λa.
          case a of
-	   m0_c b => m0_d (m0_proj s b)
+           m0_c b => m0_d (m0_proj s b)
          | m0u_c_Input => m0u_d_stream input
-	 | m0u_c_Output => m0u_d_stream output
+         | m0u_c_Output => m0u_d_stream output
          | m0u_c_RDX => m0u_d_word32 u.RXD
          | m0u_c_TXD => m0u_d_word32 u.TXD
          | m0u_c_RDXRDY => m0u_d_bool u.TXDRDY
-         | m0u_c_TXDRDY => m0u_d_bool u.RXDRDY) 
-`; 
-      
+         | m0u_c_TXDRDY => m0u_d_bool u.RXDRDY)
+`;
+
 
 val m0u_instr_def = Define`
     (m0u_instr (a,INL opc16) =
@@ -57,7 +58,7 @@ val m0u_instr_def = Define`
         (m0_c (m0_c_MEM (a + 3w)),m0_d (m0_d_word8 ((15 >< 8) opc32)))})`
 
 
-(* Translate M0 separation logit to M0U separation logic *)  
+(* Translate M0 separation logit to M0U separation logic *)
 
 (* low level mapping *)
 val TO_M0U_def = Define`
@@ -87,7 +88,7 @@ val cond_2_m0u_thm = store_thm("cond_2_m0u_thm",
 );
 
 (* m0u abrivations *)
-val instr_2_m0u_thm = store_thm( "instr_2_m0u_thm", 
+val instr_2_m0u_thm = store_thm( "instr_2_m0u_thm",
     ``TO_M0U o m0_instr = m0u_instr``,
     SIMP_TAC std_ss [FUN_EQ_THM]>>
     Cases_on `x`>> rename1 `(addr,inst)`>> Cases_on `inst`>>
@@ -98,21 +99,21 @@ val CODE_POOL_2_m0u_thm = store_thm( "CODE_POOL_2_m0u_thm",
 ``!code. TO_M0U_PROP (CODE_POOL m0_instr code) = CODE_POOL m0u_instr code``,
     FULL_SIMP_TAC (bool_ss) [TO_M0U_PROP_def, CODE_POOL_def]>>
     STRIP_TAC>>
+cheat
     (* TODO: prove cheeted lemma  *)
-    ` IMAGE (TO_M0U) (\s. s = BIGUNION (IMAGE m0_instr code))
-= (λs. s = TO_M0U (BIGUNION (IMAGE m0_instr code)))` by  cheat>>
+    (* ` IMAGE (TO_M0U) (\s. s = BIGUNION (IMAGE m0_instr code)) = (λs. s = TO_M0U (BIGUNION (IMAGE m0_instr code)))` by  cheat>>
    ASM_SIMP_TAC std_ss [TO_M0U_def, IMAGE_BIGUNION, IMAGE_IMAGE]>>
-   SIMP_TAC std_ss [GSYM TO_M0U_def, instr_2_m0u_thm]
+   SIMP_TAC std_ss [GSYM TO_M0U_def, instr_2_m0u_thm]*)
 );
 
 
 (*
 val count_2_m0u_thm = store_thm( "count_2_m0u_thm",
 ``!code. TO_M0U_PROP (m0_count) = CODE_POOL m0u_instr code``,
-                                            
+
 );*)
 
-val PROP_2_m0u_RWR  = [star_2_m0u_thm, cond_2_m0u_thm, instr_2_m0u_thm, CODE_POOL_2_m0u_thm ]
+val PROP_2_m0u_RWR  = [star_2_m0u_thm, cond_2_m0u_thm, instr_2_m0u_thm, CODE_POOL_2_m0u_thm ];
 (********************************************)
 (*        Sep logic Domain theory           *)
 (********************************************)
@@ -142,7 +143,7 @@ val m0_DOM_STAR_thm = store_thm("m0_SDOM_STAR_thm", ``
 
 (* Intuitivly it seas like this should also be true,
 
-   it colud be easer to use 
+   it colud be easer to use
  *)
 val m0_DOM_STAR_2thm = prove(``!A B.  DOM (A * B) = (DOM A) UNION (DOM B)``, cheat);
 val m0_DOM_COND_thm = prove(``!x. DOM(cond x) = {} ``, cheat);
@@ -167,11 +168,21 @@ DB.find "m0_REG"
 (*                                          *)
 (********************************************)
 
+
+val SEQ_MONO_LEM = Q.prove( `!seq s i t.
+    (rel_sequence (NEXT_REL $= NextStateM0) seq s)/\
+    ((seq (SUC i)).count < s.count + t)==> ((seq i).count < s.count + t)`,
+    REPEAT GEN_TAC>>
+    (MP_TAC o Q.SPECL[`s`,`i`,`SUC i`,`seq`] ) SEQ_MONO_B>>
+    ASM_SIMP_TAC std_ss []>>
+    METIS_TAC [ DECIDE ``( x:num <= y:num /\ y < z:num ) ==> (x < z) ``]
+);
+
 val NextStateM0U_def = Define ` NextStateM0U s0 =
       (let
         s1  = m0u_Next s0
       in
-          if (~(((SND o FST)s1).unpredictable) /\ (((FST o FST)s1).exception = NoException))
+         if ((FST o FST)s1).exception = NoException
          then SOME s1 else NONE)`;
 
 
@@ -186,52 +197,74 @@ val M0U_MODEL = Define `M0U_MODEL = (
     m0u_instr,
 
     (* equality of states *)
-    $=  :((m0_state # uart_state) # word32 list # word32 list)-> 
+    $=  :((m0_state # uart_state) # word32 list # word32 list)->
          ((m0_state # uart_state) # word32 list # word32 list)-> bool,
-    
+
     (* Not sure what this is for, it does not seem to be uneful in the m0 model *)
     K F :((m0_state # uart_state) # word32 list # word32 list)-> bool
     )`;
 
-val COSIM_def = Define ` COSIM P t = ! s s' seq seq' i.   
+
+(* ALTERNET def, might be a theorem 
+val COSIM_def = Define `COSIM P t = ! s s' seq seq' i.
     ((SEP_REFINE (P * SEP_T) ($=) (STATE m0_proj) s) /\
     rel_sequence (NEXT_REL $= NextStateM0) seq  s /\
     rel_sequence (NEXT_REL $= NextStateM0U) seq' s' /\
-    ~(((SND o FST) s').unpredictable)/\
-    m0u_m0_non_r_eq uart_r s' s /\ ((seq i).count <= s.count + t) )==>   
-	m0u_m0_non_r_eq uart_r (seq' i) (seq i) /\
-	m0u_r_eq uart_r s' (seq' i)`;
+    m0u_m0_non_r_eq uart_r s' s /\ ((seq i).count < s.count + t) )==>
+        m0u_m0_non_r_eq uart_r (seq' i) (seq i) /\
+        m0u_r_eq uart_r s' (seq' i)/\
+        m0u_m0_non_r_eq uart_r (seq' (SUC i)) (seq (SUC i)) /\
+        m0u_r_eq uart_r s' (seq' (SUC i))`;
 
+*)
+
+val COSIM_def = Define `COSIM P t = ! s s' seq seq' i.
+    ((SEP_REFINE (P * SEP_T) ($=) (STATE m0_proj) s) /\
+    rel_sequence (NEXT_REL $= NextStateM0) seq  s /\
+    rel_sequence (NEXT_REL $= NextStateM0U) seq' s' /\
+    m0u_m0_non_r_eq uart_r s' s /\ ((seq i).count < s.count + t) )==>
+        m0u_m0_non_r_eq uart_r (m0u_Next (seq' i)) (Next (seq i)) /\
+        m0u_r_eq uart_r (seq' i)  (m0u_Next (seq' i))`;
 
 val cosim_def = Define `cosim P c t = COSIM ((CODE_POOL m0_instr c) * P  ) t`;
 
 val NEX_thm = Q.store_thm("NEX_thm",
-    `! P t s seq i.
-	NEX P t ==> (
-	    SEP_REFINE (P * SEP_T) $= (STATE m0_proj) s /\
-	    rel_sequence (NEXT_REL $= NextStateM0) seq s /\
-	    (seq (SUC i)).count <= s.count + t ==> 
+    `! P t. 
+        (NEX P t) ==> (! s seq i. 
+            SEP_REFINE (P * SEP_T) $= (STATE m0_proj) s /\
+            rel_sequence (NEXT_REL $= NextStateM0) seq s /\
+            (seq (i)).count < s.count + t ==>
                 ((seq i).count < (Next(seq i)).count) /\ ((Next (seq i)) = (seq(SUC i))))`,
-    REPEAT STRIP_TAC>>
-    FULL_SIMP_TAC (std_ss++LET_ss) [NEX_def, PULL_FORALL]>>
-    Q.PAT_X_ASSUM `!s seq i._` (MP_TAC o Q.SPECL [`s`,`seq`, `i`])>>
-    FULL_SIMP_TAC (std_ss++LET_ss) [NEX_def, PULL_FORALL,rel_sequence_def, 
-			    NEXT_REL_EQ, NextStateM0_def]>>
+    REPEAT GEN_TAC>>
+    STRIP_TAC>>
+    REPEAT GEN_TAC>>
+    Induct_on `i` >- (
+        STRIP_TAC>>
+        `(seq 0).count < (Next (seq 0)).count ∧
+        ((Next (seq 0)).exception = NoException)` by METIS_TAC[NEX_def]>>
+        FULL_SIMP_TAC std_ss [NEX_def, rel_sequence_def, NEXT_REL_def, NextStateM0_def, LET_DEF]>>
+        `Next (seq 0) = seq (SUC 0)` by METIS_TAC[]>>
+        REV_FULL_SIMP_TAC std_ss []
+    )>>
+    STRIP_TAC>>
+    `(seq (SUC i)).count < (Next (seq (SUC i))).count ∧
+    ((Next (seq (SUC i))).exception = NoException)` by METIS_TAC[NEX_def, SEQ_MONO_LEM]>>
+    FULL_SIMP_TAC std_ss [NEX_def, rel_sequence_def, NEXT_REL_def, NextStateM0_def, LET_DEF]>>
     METIS_TAC[]
 );
 
 val PRODUCT_STATE_lem = prove(``!s z_i. ?z_0. m0_non_r_eq uart_r s z_0 /\ m0_r_eq uart_r z_0 z_i``,
     REPEAT GEN_TAC>>
-    EXISTS_TAC ``s with <|MEM := (\x. if (x IN uart_r) 
+    EXISTS_TAC ``s with <|MEM := (\x. if (x IN uart_r)
                                          then (z_i.MEM x)
                                          else (s.MEM x)) |>``>>
     SIMP_TAC (std_ss++pred_setLib.PRED_SET_ss) [m0Theory.m0_state_accfupds,
-		m0_non_r_eq_def, m0_r_eq_def, mem_eq_def]
+                m0_non_r_eq_def, m0_r_eq_def, mem_eq_def]
 );
 
 val eq_lem = prove(``!a b r.
     m0_non_r_eq r a  b /\ m0_r_eq r a b ==> (a=b)``,
-			      
+
     REPEAT GEN_TAC>>
     Cases_on `a`>>Cases_on `b`>>
     SIMP_TAC (std_ss++pred_setLib.PRED_SET_ss) [m0Theory.m0_state_accfupds,
@@ -239,119 +272,60 @@ m0Theory.m0_state_accessors,m0_non_r_eq_def, m0_r_eq_def, mem_eq_def, m0Theory.m
     Cases_on  `x NOTIN r ` >> METIS_TAC[]
 );
 
-val   NIT_NIT_STEP_thm = store_thm("NIT_NIT_STEP_thm",
-``  ! P t s seq i.
-	NIT uart_r P t /\
-	NEX P t ==> (
-	SEP_REFINE (P * SEP_T) $= (STATE m0_proj) s /\
-	rel_sequence (NEXT_REL $= NextStateM0) seq s /\
-	(seq (SUC i)).count <= s.count + t ==> NIT_STEP uart_r (seq i))``,
-    REPEAT STRIP_TAC >>
-    SIMP_TAC std_ss [NIT_STEP_thm]>>
-    GEN_TAC>>
-    rename1 `m0_non_r_eq uart_r (seq i) z_i`>>
-    STRIP_TAC>>
-    `?z_0. m0_non_r_eq uart_r s z_0 /\ m0_r_eq uart_r z_0 z_i` by( 
-        METIS_TAC[PRODUCT_STATE_lem]
-    )>>
-    `?seq_z . rel_sequence (NEXT_REL $= NextStateM0) seq_z z_0` by(
-        METIS_TAC[SEQUENCE_EXISTS_THM]
-    )>>
- 
-    `(seq i).count ≤ s.count + t` by(
-	METIS_TAC[NEX_thm,
-	    DECIDE ``((a:num) < (b:num) /\ b <= (c:num)) ==>( a <= c)``])>>
 
-    `z_i = seq_z i ` by (
-	Q.PAT_ASSUM `NIT uart_r P t` (MP_TAC o 
-				  Q.SPECL [`s`, `z_0`, `seq`, `seq_z`, `i`] o
-                                  REWRITE_RULE [NIT_def])>>
-	METIS_TAC[m0_r_eq_trans_thm, m0_r_eq_antisym_thm,
-                  m0_non_r_eq_trans_thm, m0_non_r_eq_antisym_thm,
-                  eq_lem])>>
-    
-    Q.PAT_ASSUM `NIT uart_r P t` (MP_TAC o 
-	   			  Q.SPECL [`s`, `z_0`, `seq`, `seq_z`, `SUC i`] o
-                                  REWRITE_RULE [NIT_def])>>
-    ASM_SIMP_TAC std_ss []>>
-    STRIP_TAC>>
-
-    `(seq(SUC i) = Next (seq(i)))` by  (METIS_TAC[NEX_thm])>>
-
-   `(seq_z(SUC i) = Next (seq_z(i)))` by(
-        (* a step must have taken place between (seq_z i) and i+1 
-           since the count between them has increesed *) 
-	`(seq_z(i)).count < (seq_z(SUC i)).count ` by
-	    METIS_TAC[NEX_thm,  m0_non_r_eq_def]>>
-	Q.PAT_X_ASSUM `rel_sequence (NEXT_REL $= NextStateM0) seq_z s_0` 
-	    (MP_TAC o Q.SPEC `i` o 
-	    SIMP_RULE (std_ss++LET_ss)[
-		rel_sequence_def, PULL_EXISTS,NEXT_REL_EQ,
-		NextStateM0_def, PULL_FORALL])>>
-         IF_CASES_TAC >-  (METIS_TAC[] )>>
-	 STRIP_TAC >> FULL_SIMP_TAC arith_ss[]
-    )>>
-    
-    METIS_TAC[m0_r_eq_trans_thm,m0_r_eq_antisym_thm]
-);
- 
 val LEM = prove(
-    ``!(a:((m0_state # uart_state) # word32 list # word32 list)) 
+    ``!(a:((m0_state # uart_state) # word32 list # word32 list))
        (b:((m0_state # uart_state) # word32 list # word32 list)) region.
-	    m0u_r_eq region a b ==> ((SND (FST a)) = (SND (FST b)))``, 
+            m0u_r_eq region a b ==> ((SND (FST a)) = (SND (FST b)))``,
     Cases_on `a`>> Cases_on `b`>> Cases_on `q`>>
     Cases_on `q'`>> Cases_on `r`>> Cases_on `r'`>>
     SIMP_TAC std_ss [m0u_r_eq_def]
 );
+
+
 val LEM1 = prove(
-    ``!a b region. (m0u_m0_non_r_eq  region a b) ==> 
-	((FST (FST a)).count =  b.count)/\
-	((FST (FST a)).exception =  b.exception)``, 
+    ``!a b region. (m0u_m0_non_r_eq  region a b) ==>
+        (((FST o FST) a).count =  b.count)/\
+        (((FST o FST) a).exception =  b.exception)``,
     Cases_on `a`>> Cases_on `q`>> Cases_on `r`>>
     SIMP_TAC std_ss [m0u_m0_non_r_eq_def, m0_non_r_eq_def]
 );
 
-val NIT_COSIM_thm = Q.store_thm ("NIT_COSIM_thm", 
-    `!P t.  ((NIT uart_r P t) /\ (NEX P t)) ==> (COSIM P t)`, 
+
+val NIT_COSIM_thm = Q.store_thm ("NIT_COSIM_thm",
+    `!P t.  ((NIT uart_r P t) /\ (NEX P t)) ==> (COSIM P t)`,
     SIMP_TAC std_ss [ COSIM_def, PULL_FORALL]>>
     REPEAT GEN_TAC>>
-    Induct_on `i`>-(
-        ASM_SIMP_TAC std_ss [rel_sequence_def, m0u_r_eq_refl_thm]
+    STRIP_TAC>>
+    STRIP_TAC>>
+    Induct_on `i` >-(
+        STRIP_TAC>>
+        `((seq 0).count < (Next (seq 0)).count) ∧( (Next (seq 0) = seq (SUC 0)))` by
+            METIS_TAC[NEX_thm]>>
+        `NIT_STEP uart_r (seq 0)` by METIS_TAC[NIT_NIT_STEP_thm]>>
+        METIS_TAC[rel_sequence_def, AXI, m0u_r_eq_antisym_thm]
     )>>
-    STRIP_TAC>>STRIP_TAC>>
-    `(seq i).count ≤ s.count + t` by(
-	METIS_TAC[NEX_thm,
-	    DECIDE ``((a:num) < (b:num) /\ b <= (c:num)) ==>( a <= c)``])>>
+    STRIP_TAC >>
+    `(seq i).count < s.count + t` by (
+        METIS_TAC[SEQ_MONO_LEM]
+    )>>
     FULL_SIMP_TAC std_ss []>>
-    (MP_TAC o Q.SPECL [`P`,`t`,`s`,`seq`, `i`]) NIT_NIT_STEP_thm>>
-    ASM_SIMP_TAC std_ss[]>>
-    STRIP_TAC>>
-    `(seq(SUC i) = Next (seq(i)))` by  (METIS_TAC[NEX_thm])>>
-    (MP_TAC o Q.SPECL [`seq (i:num)`, `seq' (i:num)`]) AXI>>
-    ASM_SIMP_TAC std_ss[]>>
-    STRIP_TAC>>
-    `seq' (SUC i) = m0u_Next (seq' i)` by (
-	`(Next (seq i)).exception = NoException` by (
-	    Q.PAT_X_ASSUM `NIX P t` ( 
-                MP_TAC o Q.SPECL [`s`, `seq`, `i`] o
-		REWRITE_RULE [NEX_def])>>
-	    FULL_SIMP_TAC std_ss []
-	)>>
-	` m0u_r_eq uart_r s' (m0u_Next (seq' i))` by(
-	    METIS_TAC [m0u_r_eq_trans_thm, m0u_r_eq_antisym_thm]
-        )>>
-	Q.PAT_X_ASSUM `rel_sequence (NEXT_REL $= NextStateM0U) seq' s'` (MP_TAC o
-	    SPEC ``i:num`` o
-	    CONJUNCT2 o
-	    REWRITE_RULE [PULL_FORALL,rel_sequence_def, 
-                          NEXT_REL_EQ, NextStateM0U_def]
-        )>>
-	ASM_SIMP_TAC (std_ss++LET_ss) []>>
-	METIS_TAC[NextStateM0U_def, LEM, LEM1]
+    ` (seq i).count < (Next (seq i)).count ∧
+    (Next (seq i) = seq (SUC i))` by METIS_TAC[NEX_thm]>>
+    ` (seq (SUC i)).count < (Next (seq (SUC i))).count ∧
+    (Next (seq (SUC i)) = seq (SUC(SUC i)))` by METIS_TAC[NEX_thm]>>
+    `NIT_STEP uart_r (seq (SUC i) )` by METIS_TAC[NIT_NIT_STEP_thm]>>
+    `m0u_Next (seq' i) =  (seq' (SUC i))` by (
+        ` ((FST ∘ FST) (m0u_Next (seq' i))).exception = NoException` by METIS_TAC[LEM1,NEX_def]>>
+        `if ∃x. NEXT_REL $= NextStateM0U (seq' i) x then
+               NEXT_REL $= NextStateM0U (seq' i) (seq' (SUC i))
+             else seq' (SUC i) = seq' i` by METIS_TAC [rel_sequence_def]>>
+        FULL_SIMP_TAC bool_ss [rel_sequence_def, NextStateM0U_def,
+                               NEXT_REL_def, LET_DEF, PULL_EXISTS]>>
+        METIS_TAC[optionTheory.option_CLAUSES, rel_sequence_def]
     )>>
-    METIS_TAC [m0u_r_eq_trans_thm,  m0u_r_eq_antisym_thm]
+    METIS_TAC [m0u_r_eq_antisym_thm, AXI]
 );
-
 (********************************************)
 (*          Transfere properties            *)
 (*                                          *)
@@ -366,18 +340,18 @@ first lemma for proving the TP theorem:
 
 seccond lemma for proving the TP theorem
 
-{P} c {Q} /\ DISJOINT (P UNION Q) UART ==> m 
+{P} c {Q} /\ DISJOINT (P UNION Q) UART ==> m
 *)
              (*
 val TP_thm = Q.store_thm("TP_thm",
-    `!P C Q c t C. 
-        (SPEC M0_MODEL (P*m0_count c) C (Q*m0_count (c+t))) /\ 
-	(cosim (P * m0_count c) C t) ==>   
-	    (SPEC M0U_MODEL (TO_M0U_PROP (P * m0_count c)) C (TO_M0U_PROP(Q * m0_count (c+t))))`,
+    `!P C Q c t C.
+        (SPEC M0_MODEL (P*m0_count c) C (Q*m0_count (c+t))) /\
+        (cosim (P * m0_count c) C t) ==>
+            (SPEC M0U_MODEL (TO_M0U_PROP (P * m0_count c)) C (TO_M0U_PROP(Q * m0_count (c+t))))`,
 
            REWRITE_TAC[SPEC_def, M0U_MODEL, RUN_def]>>
     REPEAT STRIP_TAC>>
-    
+
 
 FULL_SIMP_TAC std_ss [GSYM CODE_POOL_2_m0u_thm, GSYM star_2_m0u_thm]>>
 FULL_SIMP_TAC std_ss [cosim_def, COSIM_def]>>
@@ -390,19 +364,20 @@ FULL_SIMP_TAC std_ss [cosim_def, COSIM_def]>>
         (DISJOINT (DOM Q) UART) ==>
     REPEAT STRIP_TAC
     cheat);*)
-
+(*
 val WS_COSIM_thm = Q.store_thm("WS_COSIM_thm",
     `!P P' t t'. COSIM P t /\ t' < t  /\ (SEP_IMP P' P) ==> COSIM P' t'`,
     SIMP_TAC arith_ss [COSIM_def, PULL_FORALL]>>
     REPEAT STRIP_TAC>>(
-	Q.PAT_X_ASSUM `!s s' seq seq' i._` (MP_TAC o Q.SPECL [`s`, `s'`, `seq`, `seq'`, `i`] )>>
-	REPEAT STRIP_TAC>>
-	` (seq i).count ≤ t+s.count` by DECIDE_TAC>>
-	`SEP_REFINE (P * SEP_T) $= (STATE m0_proj) s` by (
-	REV_FULL_SIMP_TAC std_ss [SEP_IMP_def, STAR_def,SEP_REFINE_def]>>
-	METIS_TAC [])>>
-	METIS_TAC []
+        Q.PAT_X_ASSUM `!s s' seq seq' i._` (MP_TAC o Q.SPECL [`s`, `s'`, `seq`, `seq'`, `i`] )>>
+        REPEAT STRIP_TAC>>
+        ` (seq i).count ≤ t+s.count` by DECIDE_TAC>>
+        `SEP_REFINE (P * SEP_T) $= (STATE m0_proj) s` by (
+        REV_FULL_SIMP_TAC std_ss [SEP_IMP_def, STAR_def,SEP_REFINE_def]>>
+        METIS_TAC [])>>
+        METIS_TAC []
     )
 );
+*)
 
 val _ = export_theory();
